@prefix : <https://w3id.org/yang/server#> .
@prefix ys: <https://w3id.org/yang/server#> .
@prefix mod: <https://w3id.org/mod#> .
@prefix owl: <http://www.w3.org/2002/07/owl#> .
@prefix rdf: <http://www.w3.org/1999/02/22-rdf-syntax-ns#> .
@prefix rml: <http://w3id.org/rml/> .
@prefix xml: <http://www.w3.org/XML/1998/namespace> .
@prefix xsd: <http://www.w3.org/2001/XMLSchema#> .
@prefix foaf: <http://xmlns.com/foaf/0.1/> .
@prefix qudt: <http://qudt.org/schema/qudt/> .
@prefix rdfs: <http://www.w3.org/2000/01/rdf-schema#> .
@prefix vann: <http://purl.org/vocab/vann/> .
@prefix schema: <https://schema.org/> .
@prefix dcterms: <http://purl.org/dc/terms/> .
@prefix observable: <https://ontology.unifiedcyberontology.org/uco/observable/> .
@base <https://w3id.org/yang/server> .

<https://w3id.org/yang/server> rdf:type owl:Ontology ;
                                owl:versionIRI <https://w3id.org/yang/server> ;
                                dcterms:created "2025-01-08"^^xsd:date ;
                                dcterms:creator [ foaf:name "Ignacio Dominguez Martinez-Casanueva" ;
                                                  schema:identifier <https://orcid.org/0000-0002-8573-127X>
                                                ] ;
                                dcterms:description """
                                 Ontology that defines core concepts for representing YANG servers, including connection details and the available YANG datastores, along with operations for retrieving YANG data from a YANG server. The goal of this ontology is to enable the declarative and abstract of the interactions with YANG servers for monitoring and configuration purposes. In this sense, the ontology can become the basis for building a knowledge graph from YANG data obtained from YANG servers.
                                 """ ;
                                dcterms:license <http://purl.org/NET/rdflicense/APACHE2.0> ;
                                dcterms:publisher [ foaf:homepage <https://github.com/candil-data-fabric> ;
                                                    foaf:name "CANDIL Data Fabric"
                                                  ] ;
                                dcterms:source <https://github.com/candil-data-fabric/yang-server-ontology> ;
                                dcterms:title "YANG Server Ontology" ;
                                vann:preferredNamespacePrefix "ys" ;
                                vann:preferredNamespaceUri ys: ;
                                rdfs:label "YANG Server Ontology"@en ;
                                owl:versionInfo "1.5.0" ;
                                mod:createdWith <https://chowlk.linkeddata.es/> .

#################################################################
#    Annotation properties
#################################################################

###  http://purl.org/dc/terms/created
dcterms:created rdf:type owl:AnnotationProperty .


###  http://purl.org/dc/terms/creator
dcterms:creator rdf:type owl:AnnotationProperty .


###  http://purl.org/dc/terms/description
dcterms:description rdf:type owl:AnnotationProperty .


###  http://purl.org/dc/terms/license
dcterms:license rdf:type owl:AnnotationProperty .


###  http://purl.org/dc/terms/publisher
dcterms:publisher rdf:type owl:AnnotationProperty .


###  http://purl.org/dc/terms/source
dcterms:source rdf:type owl:AnnotationProperty .


###  http://purl.org/dc/terms/title
dcterms:title rdf:type owl:AnnotationProperty .


###  http://purl.org/vocab/vann/example
vann:example rdf:type owl:AnnotationProperty .


###  http://purl.org/vocab/vann/preferredNamespacePrefix
vann:preferredNamespacePrefix rdf:type owl:AnnotationProperty .


###  http://purl.org/vocab/vann/preferredNamespaceUri
vann:preferredNamespaceUri rdf:type owl:AnnotationProperty .


###  http://www.w3.org/2002/07/owl#versionInfo
owl:versionInfo rdf:type owl:AnnotationProperty .


###  http://xmlns.com/foaf/0.1/homepage
foaf:homepage rdf:type owl:AnnotationProperty .


###  http://xmlns.com/foaf/0.1/name
foaf:name rdf:type owl:AnnotationProperty .


###  https://schema.org/identifier
schema:identifier rdf:type owl:AnnotationProperty .


###  https://w3id.org/mod#createdWith
mod:createdWith rdf:type owl:AnnotationProperty .


#################################################################
#    Object Properties
#################################################################

###  http://qudt.org/schema/qudt/unit
qudt:unit rdf:type owl:ObjectProperty ;
          rdfs:range qudt:Unit ;
          rdfs:isDefinedBy <http://qudt.org/2.1/schema/qudt> ;
          rdfs:label "unit" .


###  https://w3id.org/yang/server#capability
ys:capability rdf:type owl:ObjectProperty ;
              rdfs:domain ys:NetconfServer ;
              rdfs:range ys:NetconfCapability ;
              rdfs:comment "Refers to the NETCONF capability supported by the NETCONF server." ;
              rdfs:isDefinedBy <https://w3id.org/yang/server> ;
              rdfs:label "capability" .


###  https://w3id.org/yang/server#datastore
ys:datastore rdf:type owl:ObjectProperty ;
             rdfs:domain ys:YangServer ;
             rdfs:range ys:Datastore ;
             rdfs:comment "Indicates the YANG datastore used by the YANG server." ;
             rdfs:isDefinedBy <https://w3id.org/yang/server> ;
             rdfs:label "datastore" .


###  https://w3id.org/yang/server#filter
ys:filter rdf:type owl:ObjectProperty ;
          rdfs:domain [ rdf:type owl:Class ;
                        owl:unionOf ( ys:Query
                                      ys:Subscription
                                    )
                      ] ;
          rdfs:range ys:Filter ;
          rdfs:comment "Refers to the YANG filter used when accessing the YANG server using a network management protocol." ;
          rdfs:isDefinedBy <https://w3id.org/yang/server> ;
          rdfs:label "filter" .


###  https://w3id.org/yang/server#namespace
ys:namespace rdf:type owl:ObjectProperty ;
             rdfs:domain ys:XPathFilter ;
             rdfs:range ys:Namespace ;
             rdfs:comment "Refers to an XML namespace used in the XPath expression." ;
             rdfs:isDefinedBy <https://w3id.org/yang/server> ;
             rdfs:label "namespace" .


###  https://w3id.org/yang/server#period
ys:period rdf:type owl:ObjectProperty ;
          rdfs:domain ys:PeriodicSubscription ;
          rdfs:range ys:Period ;
          rdfs:comment "Refers to period interval with which to report updates in a periodic subscription." ;
          rdfs:isDefinedBy <https://w3id.org/yang/server> ;
          rdfs:label "period" ;
          rdfs:seeAlso <https://datatracker.ietf.org/doc/rfc8641> .


###  https://w3id.org/yang/server#sourceDatastore
ys:sourceDatastore rdf:type owl:ObjectProperty ;
                   rdfs:domain [ rdf:type owl:Class ;
                                 owl:unionOf ( ys:Query
                                               ys:Subscription
                                             )
                               ] ;
                   rdfs:range ys:Datastore ;
                   rdfs:comment "Refers to the YANG datastore of the source YANG server to be selected in the YANG operation." ;
                   rdfs:isDefinedBy <https://w3id.org/yang/server> ;
                   rdfs:label "source datastore" .


###  https://w3id.org/yang/server#sourceServer
ys:sourceServer rdf:type owl:ObjectProperty ;
                rdfs:domain [ rdf:type owl:Class ;
                              owl:unionOf ( ys:Query
                                            ys:Subscription
                                          )
                            ] ;
                rdfs:range ys:YangServer ;
                rdfs:comment "Refers to the YANG server which the YANG operation is sent to using a network management protocol." ;
                rdfs:isDefinedBy <https://w3id.org/yang/server> ;
                rdfs:label "source server" .


#################################################################
#    Data properties
#################################################################

###  http://purl.org/dc/terms/identifier
dcterms:identifier rdf:type owl:DatatypeProperty ;
                   rdfs:domain ys:NetconfCapability ;
                   rdfs:range xsd:string ;
                   rdfs:isDefinedBy dcterms: ;
                   rdfs:label "identifier" .


###  http://qudt.org/schema/qudt/numericValue
qudt:numericValue rdf:type owl:DatatypeProperty ;
                  rdfs:isDefinedBy <http://qudt.org/2.1/schema/qudt> ;
                  rdfs:label "numeric value" .


###  http://xmlns.com/foaf/0.1/accountName
foaf:accountName rdf:type owl:DatatypeProperty ;
                 rdfs:isDefinedBy foaf: ;
                 rdfs:label "account name" .


###  https://ontology.unifiedcyberontology.org/uco/observable/userName
observable:userName rdf:type owl:DatatypeProperty ;
                    rdfs:isDefinedBy observable: ;
                    rdfs:label "userName" .


###  https://w3id.org/yang/server#endpoint
ys:endpoint rdf:type owl:DatatypeProperty ;
            rdfs:domain ys:YangServer ;
            rdfs:range xsd:string ;
            vann:example "192.168.1.10:830" ;
            rdfs:comment "YANG server endpoint. " ;
            rdfs:isDefinedBy <https://w3id.org/yang/server> ;
            rdfs:label "endpoint" .


###  https://w3id.org/yang/server#filterValue
ys:filterValue rdf:type owl:DatatypeProperty ;
               rdfs:domain ys:Filter ;
               rdfs:range xsd:string ;
               rdfs:comment "Value used by filter to access YANG data of the NETCONF server." ;
               rdfs:isDefinedBy <https://w3id.org/yang/server> ;
               rdfs:label "filter value" ;
               rdfs:seeAlso <https://datatracker.ietf.org/doc/rfc6241> .


###  https://w3id.org/yang/server#hostKeyVerification
ys:hostKeyVerification rdf:type owl:DatatypeProperty ;
                       rdfs:domain ys:NetconfServer ;
                       rdfs:range xsd:boolean ;
                       rdfs:comment "Indicates whether SSH host key is verified to access the NETCONF server." ;
                       rdfs:isDefinedBy <https://w3id.org/yang/server> ;
                       rdfs:label "host key verification" .


###  https://w3id.org/yang/server#namespacePrefix
ys:namespacePrefix rdf:type owl:DatatypeProperty ;
                   rdfs:domain ys:Namespace ;
                   rdfs:range xsd:string ;
                   rdfs:comment "Prefix of the XML namespace." ;
                   rdfs:isDefinedBy <https://w3id.org/yang/server> ;
                   rdfs:label "namespace prefix" .


###  https://w3id.org/yang/server#namespaceURL
ys:namespaceURL rdf:type owl:DatatypeProperty ;
                rdfs:domain ys:Namespace ;
                rdfs:range xsd:anyURI ;
                rdfs:comment "URL of the XML namespace." ;
                rdfs:isDefinedBy <https://w3id.org/yang/server> ;
                rdfs:label "namespace url" .


###  https://w3id.org/yang/server#subtreeValue
ys:subtreeValue rdf:type owl:DatatypeProperty ;
                rdfs:subPropertyOf ys:filterValue ;
                rdfs:domain ys:SubtreeFilter ;
                rdfs:range rdf:XMLLiteral ;
                rdfs:comment "XML Subtree filter used to access YANG data of the NETCONF server." ;
                rdfs:isDefinedBy <https://w3id.org/yang/server> ;
                rdfs:label "subtree value" .


###  https://w3id.org/yang/server#username
ys:username rdf:type owl:DatatypeProperty ;
            rdfs:subPropertyOf foaf:accountName ,
                               observable:userName ;
            rdfs:domain ys:ServerAccount ;
            rdfs:range xsd:string ;
            rdfs:comment "Username for accessing the YANG server." ;
            rdfs:isDefinedBy <https://w3id.org/yang/server> ;
            rdfs:label "username" .


###  https://w3id.org/yang/server#xpathValue
ys:xpathValue rdf:type owl:DatatypeProperty ;
              rdfs:subPropertyOf ys:filterValue ;
              rdfs:domain ys:XPathFilter ;
              rdfs:range xsd:string ;
              vann:example "/ietf-interfaces:interfaces-state/interface" ;
              rdfs:comment "XPath expression used to access YANG data of the YANG server." ;
              rdfs:isDefinedBy <https://w3id.org/yang/server> ;
              rdfs:label "xpath value" .


#################################################################
#    Classes
#################################################################

###  http://qudt.org/schema/qudt/Unit
qudt:Unit rdf:type owl:Class ;
          rdfs:isDefinedBy <http://qudt.org/2.1/schema/qudt> ;
          rdfs:label "Unit" .


###  http://xmlns.com/foaf/0.1/OnlineAccount
foaf:OnlineAccount rdf:type owl:Class ;
                   rdfs:isDefinedBy foaf: ;
                   rdfs:label "Online Account" .


###  https://ontology.unifiedcyberontology.org/uco/observable/UserAccount
observable:UserAccount rdf:type owl:Class ;
                       rdfs:isDefinedBy observable: ;
                       rdfs:label "UserAccount" .


###  https://w3id.org/yang/server#CandidateDatastore
ys:CandidateDatastore rdf:type owl:Class ;
                      rdfs:subClassOf ys:ConventionalDatastore ;
                      rdfs:comment "A configuration datastore that can be manipulated without impacting the device's running configuration datastore and that can be committed to the running configuration datastore." ;
                      rdfs:isDefinedBy <https://w3id.org/yang/server> ;
                      rdfs:label "Candidate Datastore" ;
                      rdfs:seeAlso <https://datatracker.ietf.org/doc/rfc8342> .


###  https://w3id.org/yang/server#ConventionalDatastore
ys:ConventionalDatastore rdf:type owl:Class ;
                         rdfs:subClassOf ys:Datastore ;
                         rdfs:comment "One of the following set of configuration datastores: <running>, <startup>, <candidate>, and <intended>.  These datastores share a common datastore schema, and protocol operations allow copying data between these datastores. The term \"conventional\" is chosen as a generic umbrella term for these datastores." ;
                         rdfs:isDefinedBy <https://w3id.org/yang/server> ;
                         rdfs:label "Conventional Datastore" ;
                         rdfs:seeAlso <https://datatracker.ietf.org/doc/rfc8342> .


###  https://w3id.org/yang/server#Datastore
ys:Datastore rdf:type owl:Class ;
             rdfs:comment "A conceptual place to store and access information. A datastore might be implemented, for example, using files, a database, flash memory locations, or combinations thereof. A datastore maps to an instantiated YANG data tree." ;
             rdfs:isDefinedBy <https://w3id.org/yang/server> ;
             rdfs:label "Datastore" ;
             rdfs:seeAlso <https://datatracker.ietf.org/doc/rfc8342> .


###  https://w3id.org/yang/server#DynamicDatastore
ys:DynamicDatastore rdf:type owl:Class ;
                    rdfs:subClassOf ys:Datastore ;
                    rdfs:comment "A configuration datastore holding configuration obtained dynamically during the operation of a device through interaction with other systems, rather than through one of the conventional configuration datastores." ;
                    rdfs:isDefinedBy <https://w3id.org/yang/server> ;
                    rdfs:label "Dynamic Datastore" ;
                    rdfs:seeAlso <https://datatracker.ietf.org/doc/rfc8342> .


###  https://w3id.org/yang/server#Filter
ys:Filter rdf:type owl:Class ;
          rdfs:comment "Evaluation criteria that may be applied to fetch data from a given YANG server." ;
          rdfs:isDefinedBy <https://w3id.org/yang/server> ;
          rdfs:label "Filter" ;
          rdfs:seeAlso <https://datatracker.ietf.org/doc/rfc6241> .


###  https://w3id.org/yang/server#IntendedDatastore
ys:IntendedDatastore rdf:type owl:Class ;
                     rdfs:subClassOf ys:ConventionalDatastore ;
                     rdfs:comment "A configuration datastore holding the complete intended configuration of the device. This represents the configuration after all configuration transformations to <running> have been performed and is the configuration that the system attempts to apply." ;
                     rdfs:isDefinedBy <https://w3id.org/yang/server> ;
                     rdfs:label "Intended Datastore" ;
                     rdfs:seeAlso <https://datatracker.ietf.org/doc/rfc8342> .


###  https://w3id.org/yang/server#Namespace
ys:Namespace rdf:type owl:Class ;
             rdfs:comment "Represents an XML namespace used in the XPath expression." ;
             rdfs:isDefinedBy <https://w3id.org/yang/server> ;
             rdfs:label "Namespace" .


###  https://w3id.org/yang/server#NetconfCapability
ys:NetconfCapability rdf:type owl:Class ;
                     rdfs:comment "NETCONF capability." ;
                     rdfs:isDefinedBy <https://w3id.org/yang/server> ;
                     rdfs:label "Netconf Capability" ;
                     rdfs:seeAlso <https://datatracker.ietf.org/doc/rfc6241> .


###  https://w3id.org/yang/server#NetconfServer
ys:NetconfServer rdf:type owl:Class ;
                 rdfs:subClassOf ys:YangServer ;
                 rdfs:comment "YANG server that can be managed via the NETCONF protocol." ;
                 rdfs:isDefinedBy <https://w3id.org/yang/server> ;
                 rdfs:label "Netconf Server" ;
                 rdfs:seeAlso <https://datatracker.ietf.org/doc/rfc6241> .


###  https://w3id.org/yang/server#OnChangeSubscription
ys:OnChangeSubscription rdf:type owl:Class ;
                        rdfs:subClassOf ys:Subscription ;
                        rdfs:comment "A datastore subscription with updates that are triggered when changes in subscribed datastore nodes are detected." ;
                        rdfs:isDefinedBy <https://w3id.org/yang/server> ;
                        rdfs:label "On-change Subscription" ;
                        rdfs:seeAlso <https://datatracker.ietf.org/doc/rfc8641> .


###  https://w3id.org/yang/server#OperationalDatastore
ys:OperationalDatastore rdf:type owl:Class ;
                        rdfs:subClassOf ys:Datastore ;
                        rdfs:comment "A datastore holding the complete operational state of the device." ;
                        rdfs:isDefinedBy <https://w3id.org/yang/server> ;
                        rdfs:label "Operational Datastore" ;
                        rdfs:seeAlso <https://datatracker.ietf.org/doc/rfc8342> .


###  https://w3id.org/yang/server#Period
ys:Period rdf:type owl:Class ;
          rdfs:comment "Represents the period interval with which to report updates in a periodic subscription." ;
          rdfs:isDefinedBy <https://w3id.org/yang/server> ;
          rdfs:label "Period" ;
          rdfs:seeAlso <https://datatracker.ietf.org/doc/rfc8641> .


###  https://w3id.org/yang/server#PeriodicSubscription
ys:PeriodicSubscription rdf:type owl:Class ;
                        rdfs:subClassOf ys:Subscription ;
                        rdfs:comment "A datastore subscription with updates that are triggered periodically according to some time interval." ;
                        rdfs:isDefinedBy <https://w3id.org/yang/server> ;
                        rdfs:label "Periodic Subscription" ;
                        rdfs:seeAlso <https://datatracker.ietf.org/doc/rfc8641> .


###  https://w3id.org/yang/server#Query
ys:Query rdf:type owl:Class ;
         rdfs:comment "Represents a query operation to a YANG server using the corresponding network management protocol." ;
         rdfs:isDefinedBy <https://w3id.org/yang/server> ;
         rdfs:label "Query" ;
         rdfs:seeAlso <https://datatracker.ietf.org/doc/rfc6241> .


###  https://w3id.org/yang/server#RunningDatastore
ys:RunningDatastore rdf:type owl:Class ;
                    rdfs:subClassOf ys:ConventionalDatastore ;
                    rdfs:comment "A configuration datastore holding the current configuration of the device.  It may include configuration that requires further transformations before it can be applied." ;
                    rdfs:isDefinedBy <https://w3id.org/yang/server> ;
                    rdfs:label "Running Datastore" ;
                    rdfs:seeAlso <https://datatracker.ietf.org/doc/rfc8342> .


###  https://w3id.org/yang/server#ServerAccount
ys:ServerAccount rdf:type owl:Class ;
                 rdfs:subClassOf foaf:OnlineAccount ,
                                 observable:UserAccount ;
                 rdfs:comment "Represents an account used for accessing the YANG server." ;
                 rdfs:isDefinedBy <https://w3id.org/yang/server> ;
                 rdfs:label "Server Account" ;
                 rdfs:seeAlso <https://datatracker.ietf.org/doc/rfc6241> .


###  https://w3id.org/yang/server#StartupDatastore
ys:StartupDatastore rdf:type owl:Class ;
                    rdfs:subClassOf ys:ConventionalDatastore ;
                    rdfs:comment "A configuration datastore holding the configuration loaded by the device into the running configuration datastore when it boots." ;
                    rdfs:isDefinedBy <https://w3id.org/yang/server> ;
                    rdfs:label "Startup Datastore" ;
                    rdfs:seeAlso <https://datatracker.ietf.org/doc/rfc8342> .


###  https://w3id.org/yang/server#Subscription
ys:Subscription rdf:type owl:Class ;
                rdfs:comment "Represents a subscription operation to a YANG server using the corresponding network management protocol." ;
                rdfs:isDefinedBy <https://w3id.org/yang/server> ;
                rdfs:label "Subscription" ;
                rdfs:seeAlso <https://datatracker.ietf.org/doc/rfc8641> .


###  https://w3id.org/yang/server#SubtreeFilter
ys:SubtreeFilter rdf:type owl:Class ;
                 rdfs:subClassOf ys:Filter ;
                 rdfs:comment "Evaluation criteria based on XML subtree expression." ;
                 rdfs:isDefinedBy <https://w3id.org/yang/server> ;
                 rdfs:label "Subtree Filter" ;
                 rdfs:seeAlso <https://datatracker.ietf.org/doc/rfc6241> .


###  https://w3id.org/yang/server#XPathFilter
ys:XPathFilter rdf:type owl:Class ;
               rdfs:subClassOf ys:Filter ;
               rdfs:comment "Evaluation criteria based on XPath expression." ;
               rdfs:isDefinedBy <https://w3id.org/yang/server> ;
               rdfs:label "XPath Filter" ;
               rdfs:seeAlso <https://datatracker.ietf.org/doc/rfc6241> .


###  https://w3id.org/yang/server#YangServer
ys:YangServer rdf:type owl:Class ;
              rdfs:comment "An entity that provides access to YANG-defined data to a client, over some network management protocol." ;
              rdfs:isDefinedBy <https://w3id.org/yang/server> ;
              rdfs:label "Yang Server" ;
              rdfs:seeAlso <https://datatracker.ietf.org/doc/rfc7950> .


#################################################################
#    Individuals
#################################################################

###  https://w3id.org/yang/server#CandidateCapability
ys:CandidateCapability rdf:type owl:NamedIndividual ,
                                ys:NetconfCapability ;
                       dcterms:identifier "urn:ietf:params:netconf:capability:candidate:1.0" ;
                       rdfs:comment "The candidate configuration capability, `:candidate`, indicates that the device supports a candidate configuration datastore, which is used to hold configuration data that can be manipulated without impacting the device's current configuration." ;
                       rdfs:isDefinedBy <https://w3id.org/yang/server> ;
                       rdfs:label "Candidate Capability" ;
                       rdfs:seeAlso <https://datatracker.ietf.org/doc/html/rfc6241#section-8.3> .


###  https://w3id.org/yang/server#ConfirmedCommitCapability
ys:ConfirmedCommitCapability rdf:type owl:NamedIndividual ,
                                      ys:NetconfCapability ;
                             dcterms:identifier "urn:ietf:params:netconf:capability:confirmed-commit:1.1" ;
                             rdfs:comment "The `:confirmed-commit:1.1` capability indicates that the server will support the `<cancel-commit>` operation and the `<confirmed>`, `<confirm-timeout>`, `<persist>`, and `<persist-id>` parameters for the `<commit>` operation." ;
                             rdfs:isDefinedBy <https://w3id.org/yang/server> ;
                             rdfs:label "Confirmed Commit Capability" ;
                             rdfs:seeAlso <https://datatracker.ietf.org/doc/html/rfc6241#section-8.4> .


###  https://w3id.org/yang/server#DistinctStartupCapability
ys:DistinctStartupCapability rdf:type owl:NamedIndividual ,
                                      ys:NetconfCapability ;
                             dcterms:identifier "urn:ietf:params:netconf:capability:startup:1.0" ;
                             rdfs:comment "The device supports separate running and startup configuration datastores. The startup configuration is loaded by the device when it boots." ;
                             rdfs:isDefinedBy <https://w3id.org/yang/server> ;
                             rdfs:label "Distinct Startup Capability" ;
                             rdfs:seeAlso <https://datatracker.ietf.org/doc/html/rfc6241#section-8.7> .


###  https://w3id.org/yang/server#RollbackOnErrorCapability
ys:RollbackOnErrorCapability rdf:type owl:NamedIndividual ,
                                      ys:NetconfCapability ;
                             dcterms:identifier "urn:ietf:params:netconf:capability:rollback-on-error:1.0" ;
                             rdfs:comment "This capability indicates that the server will support the `rollback-on-error` value in the `<error-option>` parameter to the `<edit-config>` operation." ;
                             rdfs:isDefinedBy <https://w3id.org/yang/server> ;
                             rdfs:label "Rollback-on-Error Capability" ;
                             rdfs:seeAlso <https://datatracker.ietf.org/doc/html/rfc6241#section-8.5> .


###  https://w3id.org/yang/server#UrlCapability
ys:UrlCapability rdf:type owl:NamedIndividual ,
                          ys:NetconfCapability ;
                 dcterms:identifier "urn:ietf:params:netconf:capability:url:1.0" ;
                 rdfs:comment "The NETCONF peer has the ability to accept the `<url>` element in `<source>` and `<target>` parameters. The capability is further identified by URL arguments indicating the URL schemes supported." ;
                 rdfs:isDefinedBy <https://w3id.org/yang/server> ;
                 rdfs:label "URL Capability" ;
                 rdfs:seeAlso <https://datatracker.ietf.org/doc/html/rfc6241#section-8.8> .


###  https://w3id.org/yang/server#ValidationCapability
ys:ValidationCapability rdf:type owl:NamedIndividual ,
                                 ys:NetconfCapability ;
                        dcterms:identifier "urn:ietf:params:netconf:capability:validate:1.1" ;
                        rdfs:comment "Validation consists of checking a complete configuration for syntactical and semantic errors before applying the configuration to the device." ;
                        rdfs:isDefinedBy <https://w3id.org/yang/server> ;
                        rdfs:label "Validation Capability" ;
                        rdfs:seeAlso <https://datatracker.ietf.org/doc/html/rfc6241#section-8.6> .


###  https://w3id.org/yang/server#WritableRunningCapability
ys:WritableRunningCapability rdf:type owl:NamedIndividual ,
                                      ys:NetconfCapability ;
                             dcterms:identifier "urn:ietf:params:netconf:capability:writable-running:1.0" ;
                             rdfs:comment "The `:writable-running` capability indicates that the device supports direct writes to the `<running>` configuration datastore. In other words, the device supports `<edit-config>` and `<copy-config>` operations where the `<running>` configuration is the target." ;
                             rdfs:isDefinedBy <https://w3id.org/yang/server> ;
                             rdfs:label "Writable Running Capability" ;
                             rdfs:seeAlso <https://datatracker.ietf.org/doc/html/rfc6241#section-8.2> .


###  https://w3id.org/yang/server#XpathCapability
ys:XpathCapability rdf:type owl:NamedIndividual ,
                            ys:NetconfCapability ;
                   dcterms:identifier "urn:ietf:params:netconf:capability:xpath:1.0" ;
                   rdfs:comment "The XPath capability indicates that the NETCONF peer supports the use of XPath expressions in the `<filter>` element." ;
                   rdfs:isDefinedBy <https://w3id.org/yang/server> ;
                   rdfs:label "XPath Capability" ;
                   rdfs:seeAlso <https://datatracker.ietf.org/doc/html/rfc6241#section-8.9> .


###  https://w3id.org/yang/server#YangLibraryCapability
ys:YangLibraryCapability rdf:type owl:NamedIndividual ,
                                  ys:NetconfCapability ;
                         dcterms:identifier "urn:ietf:params:netconf:capability:yang-library:1.1" ;
                         rdfs:comment "NETCONF capability that indicates that the NETCONF server implements YANG Library." ;
                         rdfs:isDefinedBy <https://w3id.org/yang/server> ;
                         rdfs:label "Yang Library Capability" ;
                         rdfs:seeAlso <https://datatracker.ietf.org/doc/html/rfc8526> .

###  Generated by the OWL API (version 4.5.9.2019-02-01T07:24:44Z) https://github.com/owlcs/owlapi
