<?xml version="1.0"?>
<rdf:RDF xmlns="https://w3id.org/yang/server#"
     xml:base="https://w3id.org/yang/server"
     xmlns:mod="https://w3id.org/mod#"
     xmlns:owl="http://www.w3.org/2002/07/owl#"
     xmlns:rdf="http://www.w3.org/1999/02/22-rdf-syntax-ns#"
     xmlns:xml="http://www.w3.org/XML/1998/namespace"
     xmlns:xsd="http://www.w3.org/2001/XMLSchema#"
     xmlns:foaf="http://xmlns.com/foaf/0.1/"
     xmlns:rdfs="http://www.w3.org/2000/01/rdf-schema#"
     xmlns:vann="http://purl.org/vocab/vann/"
     xmlns:terms="http://purl.org/dc/terms/"
     xmlns:schema="https://schema.org/">
    <owl:Ontology rdf:about="https://w3id.org/yang/server">
        <owl:versionIRI rdf:resource="https://w3id.org/yang/server"/>
        <terms:created rdf:datatype="http://www.w3.org/2001/XMLSchema#date">2024-10-03</terms:created>
        <terms:creator rdf:nodeID="genid1"/>
        <terms:description>
                                 Ontology that defines core concepts for representing YANG servers, including connection details and the available YANG datastores, along with operations for retrieving YANG data from a YANG server. The goal of this ontology is to enable the declarative and abstract of the interactions with YANG servers for monitoring and configuration purposes. In this sense, the ontology can become the basis for building a knowledge graph from YANG data obtained from YANG servers.
                                 </terms:description>
        <terms:license rdf:resource="http://purl.org/NET/rdflicense/APACHE2.0"/>
        <terms:publisher rdf:nodeID="genid2"/>
        <terms:source rdf:resource="https://github.com/candil-data-fabric/yang-server-ontology"/>
        <terms:title>YANG Server Ontology</terms:title>
        <vann:preferredNamespacePrefix>ys</vann:preferredNamespacePrefix>
        <vann:preferredNamespaceUri rdf:resource="https://w3id.org/yang/server#"/>
        <rdfs:label xml:lang="en">YANG Server Ontology</rdfs:label>
        <owl:versionInfo>1.4.1</owl:versionInfo>
        <mod:createdWith rdf:resource="https://chowlk.linkeddata.es/"/>
    </owl:Ontology>
    <rdf:Description rdf:nodeID="genid1">
        <foaf:name>Ignacio Dominguez Martinez-Casanueva</foaf:name>
        <schema:identifier rdf:resource="https://orcid.org/0000-0002-8573-127X"/>
    </rdf:Description>
    <rdf:Description rdf:nodeID="genid2">
        <foaf:homepage rdf:resource="https://github.com/candil-data-fabric"/>
        <foaf:name>CANDIL Data Fabric</foaf:name>
    </rdf:Description>
    


    <!-- 
    ///////////////////////////////////////////////////////////////////////////////////////
    //
    // Annotation properties
    //
    ///////////////////////////////////////////////////////////////////////////////////////
     -->


    


    <!-- http://purl.org/dc/terms/created -->


    <owl:AnnotationProperty rdf:about="http://purl.org/dc/terms/created"/>
    


    <!-- http://purl.org/dc/terms/creator -->


    <owl:AnnotationProperty rdf:about="http://purl.org/dc/terms/creator"/>
    


    <!-- http://purl.org/dc/terms/description -->


    <owl:AnnotationProperty rdf:about="http://purl.org/dc/terms/description"/>
    


    <!-- http://purl.org/dc/terms/license -->


    <owl:AnnotationProperty rdf:about="http://purl.org/dc/terms/license"/>
    


    <!-- http://purl.org/dc/terms/publisher -->


    <owl:AnnotationProperty rdf:about="http://purl.org/dc/terms/publisher"/>
    


    <!-- http://purl.org/dc/terms/source -->


    <owl:AnnotationProperty rdf:about="http://purl.org/dc/terms/source"/>
    


    <!-- http://purl.org/dc/terms/title -->


    <owl:AnnotationProperty rdf:about="http://purl.org/dc/terms/title"/>
    


    <!-- http://purl.org/vocab/vann/example -->


    <owl:AnnotationProperty rdf:about="http://purl.org/vocab/vann/example"/>
    


    <!-- http://purl.org/vocab/vann/preferredNamespacePrefix -->


    <owl:AnnotationProperty rdf:about="http://purl.org/vocab/vann/preferredNamespacePrefix"/>
    


    <!-- http://purl.org/vocab/vann/preferredNamespaceUri -->


    <owl:AnnotationProperty rdf:about="http://purl.org/vocab/vann/preferredNamespaceUri"/>
    


    <!-- http://www.w3.org/2002/07/owl#versionInfo -->


    <owl:AnnotationProperty rdf:about="http://www.w3.org/2002/07/owl#versionInfo"/>
    


    <!-- http://xmlns.com/foaf/0.1/homepage -->


    <owl:AnnotationProperty rdf:about="http://xmlns.com/foaf/0.1/homepage"/>
    


    <!-- http://xmlns.com/foaf/0.1/name -->


    <owl:AnnotationProperty rdf:about="http://xmlns.com/foaf/0.1/name"/>
    


    <!-- https://schema.org/identifier -->


    <owl:AnnotationProperty rdf:about="https://schema.org/identifier"/>
    


    <!-- https://w3id.org/mod#createdWith -->


    <owl:AnnotationProperty rdf:about="https://w3id.org/mod#createdWith"/>
    


    <!-- 
    ///////////////////////////////////////////////////////////////////////////////////////
    //
    // Datatypes
    //
    ///////////////////////////////////////////////////////////////////////////////////////
     -->


    


    <!-- http://www.w3.org/2001/XMLSchema#date -->


    <rdfs:Datatype rdf:about="http://www.w3.org/2001/XMLSchema#date"/>
    


    <!-- 
    ///////////////////////////////////////////////////////////////////////////////////////
    //
    // Object Properties
    //
    ///////////////////////////////////////////////////////////////////////////////////////
     -->


    


    <!-- http://qudt.org/schema/qudt/unit -->


    <owl:ObjectProperty rdf:about="http://qudt.org/schema/qudt/unit">
        <rdfs:range rdf:resource="http://qudt.org/schema/qudt/Unit"/>
        <rdfs:isDefinedBy rdf:resource="http://qudt.org/2.1/schema/qudt"/>
        <rdfs:label>unit</rdfs:label>
    </owl:ObjectProperty>
    


    <!-- https://w3id.org/yang/server#capability -->


    <owl:ObjectProperty rdf:about="https://w3id.org/yang/server#capability">
        <rdfs:domain rdf:resource="https://w3id.org/yang/server#NetconfServer"/>
        <rdfs:range rdf:resource="https://w3id.org/yang/server#NetconfCapability"/>
        <rdfs:comment>Refers to the NETCONF capability supported by the NETCONF server.</rdfs:comment>
        <rdfs:isDefinedBy rdf:resource="https://w3id.org/yang/server"/>
        <rdfs:label>capability</rdfs:label>
    </owl:ObjectProperty>
    


    <!-- https://w3id.org/yang/server#datastore -->


    <owl:ObjectProperty rdf:about="https://w3id.org/yang/server#datastore">
        <rdfs:domain rdf:resource="https://w3id.org/yang/server#YangServer"/>
        <rdfs:range rdf:resource="https://w3id.org/yang/server#Datastore"/>
        <rdfs:comment>Indicates the YANG datastore used by the YANG server.</rdfs:comment>
        <rdfs:isDefinedBy rdf:resource="https://w3id.org/yang/server"/>
        <rdfs:label>datastore</rdfs:label>
    </owl:ObjectProperty>
    


    <!-- https://w3id.org/yang/server#filter -->


    <owl:ObjectProperty rdf:about="https://w3id.org/yang/server#filter">
        <rdfs:domain>
            <owl:Class>
                <owl:unionOf rdf:parseType="Collection">
                    <rdf:Description rdf:about="https://w3id.org/yang/server#Query"/>
                    <rdf:Description rdf:about="https://w3id.org/yang/server#Subscription"/>
                </owl:unionOf>
            </owl:Class>
        </rdfs:domain>
        <rdfs:range rdf:resource="https://w3id.org/yang/server#Filter"/>
        <rdfs:comment>Refers to the YANG filter used when accessing the YANG server using a network management protocol.</rdfs:comment>
        <rdfs:isDefinedBy rdf:resource="https://w3id.org/yang/server"/>
        <rdfs:label>filter</rdfs:label>
    </owl:ObjectProperty>
    


    <!-- https://w3id.org/yang/server#namespace -->


    <owl:ObjectProperty rdf:about="https://w3id.org/yang/server#namespace">
        <rdfs:domain rdf:resource="https://w3id.org/yang/server#XPathFilter"/>
        <rdfs:range rdf:resource="https://w3id.org/yang/server#Namespace"/>
        <rdfs:comment>Refers to an XML namespace used in the XPath expression.</rdfs:comment>
        <rdfs:isDefinedBy rdf:resource="https://w3id.org/yang/server"/>
        <rdfs:label>namespace</rdfs:label>
    </owl:ObjectProperty>
    


    <!-- https://w3id.org/yang/server#period -->


    <owl:ObjectProperty rdf:about="https://w3id.org/yang/server#period">
        <rdfs:domain rdf:resource="https://w3id.org/yang/server#PeriodicSubscription"/>
        <rdfs:range rdf:resource="https://w3id.org/yang/server#Period"/>
        <rdfs:comment>Refers to period interval with which to report updates in a periodic subscription.</rdfs:comment>
        <rdfs:isDefinedBy rdf:resource="https://w3id.org/yang/server"/>
        <rdfs:label>period</rdfs:label>
        <rdfs:seeAlso rdf:resource="https://datatracker.ietf.org/doc/rfc8641"/>
    </owl:ObjectProperty>
    


    <!-- https://w3id.org/yang/server#sourceDatastore -->


    <owl:ObjectProperty rdf:about="https://w3id.org/yang/server#sourceDatastore">
        <rdfs:domain>
            <owl:Class>
                <owl:unionOf rdf:parseType="Collection">
                    <rdf:Description rdf:about="https://w3id.org/yang/server#Query"/>
                    <rdf:Description rdf:about="https://w3id.org/yang/server#Subscription"/>
                </owl:unionOf>
            </owl:Class>
        </rdfs:domain>
        <rdfs:range rdf:resource="https://w3id.org/yang/server#Datastore"/>
        <rdfs:comment>Refers to the YANG datastore of the source YANG server to be selected in the YANG operation.</rdfs:comment>
        <rdfs:isDefinedBy rdf:resource="https://w3id.org/yang/server"/>
        <rdfs:label>source datastore</rdfs:label>
    </owl:ObjectProperty>
    


    <!-- https://w3id.org/yang/server#sourceServer -->


    <owl:ObjectProperty rdf:about="https://w3id.org/yang/server#sourceServer">
        <rdfs:domain>
            <owl:Class>
                <owl:unionOf rdf:parseType="Collection">
                    <rdf:Description rdf:about="https://w3id.org/yang/server#Query"/>
                    <rdf:Description rdf:about="https://w3id.org/yang/server#Subscription"/>
                </owl:unionOf>
            </owl:Class>
        </rdfs:domain>
        <rdfs:range rdf:resource="https://w3id.org/yang/server#YangServer"/>
        <rdfs:comment>Refers to the YANG server which the YANG operation is sent to using a network management protocol.</rdfs:comment>
        <rdfs:isDefinedBy rdf:resource="https://w3id.org/yang/server"/>
        <rdfs:label>source server</rdfs:label>
    </owl:ObjectProperty>
    


    <!-- 
    ///////////////////////////////////////////////////////////////////////////////////////
    //
    // Data properties
    //
    ///////////////////////////////////////////////////////////////////////////////////////
     -->


    


    <!-- http://purl.org/dc/terms/identifier -->


    <owl:DatatypeProperty rdf:about="http://purl.org/dc/terms/identifier">
        <rdfs:domain rdf:resource="https://w3id.org/yang/server#NetconfCapability"/>
        <rdfs:range rdf:resource="http://www.w3.org/2001/XMLSchema#string"/>
        <rdfs:isDefinedBy rdf:resource="http://purl.org/dc/terms/"/>
        <rdfs:label>identifier</rdfs:label>
    </owl:DatatypeProperty>
    


    <!-- http://qudt.org/schema/qudt/numericValue -->


    <owl:DatatypeProperty rdf:about="http://qudt.org/schema/qudt/numericValue">
        <rdfs:isDefinedBy rdf:resource="http://qudt.org/2.1/schema/qudt"/>
        <rdfs:label>numeric value</rdfs:label>
    </owl:DatatypeProperty>
    


    <!-- https://w3id.org/yang/server#endpoint -->


    <owl:DatatypeProperty rdf:about="https://w3id.org/yang/server#endpoint">
        <rdfs:domain rdf:resource="https://w3id.org/yang/server#YangServer"/>
        <rdfs:range rdf:resource="http://www.w3.org/2001/XMLSchema#string"/>
        <vann:example>192.168.1.10:830</vann:example>
        <rdfs:comment>YANG server endpoint. </rdfs:comment>
        <rdfs:isDefinedBy rdf:resource="https://w3id.org/yang/server"/>
        <rdfs:label>endpoint</rdfs:label>
    </owl:DatatypeProperty>
    


    <!-- https://w3id.org/yang/server#filterValue -->


    <owl:DatatypeProperty rdf:about="https://w3id.org/yang/server#filterValue">
        <rdfs:domain rdf:resource="https://w3id.org/yang/server#Filter"/>
        <rdfs:range rdf:resource="http://www.w3.org/2001/XMLSchema#string"/>
        <rdfs:comment>Value used by filter to access YANG data of the NETCONF server.</rdfs:comment>
        <rdfs:isDefinedBy rdf:resource="https://w3id.org/yang/server"/>
        <rdfs:label>filter value</rdfs:label>
        <rdfs:seeAlso rdf:resource="https://datatracker.ietf.org/doc/rfc6241"/>
    </owl:DatatypeProperty>
    


    <!-- https://w3id.org/yang/server#hostKeyVerification -->


    <owl:DatatypeProperty rdf:about="https://w3id.org/yang/server#hostKeyVerification">
        <rdfs:domain rdf:resource="https://w3id.org/yang/server#NetconfServer"/>
        <rdfs:range rdf:resource="http://www.w3.org/2001/XMLSchema#boolean"/>
        <rdfs:comment>Indicates whether SSH host key is verified to access the NETCONF server.</rdfs:comment>
        <rdfs:isDefinedBy rdf:resource="https://w3id.org/yang/server"/>
        <rdfs:label>host key verification</rdfs:label>
    </owl:DatatypeProperty>
    


    <!-- https://w3id.org/yang/server#namespacePrefix -->


    <owl:DatatypeProperty rdf:about="https://w3id.org/yang/server#namespacePrefix">
        <rdfs:domain rdf:resource="https://w3id.org/yang/server#Namespace"/>
        <rdfs:range rdf:resource="http://www.w3.org/2001/XMLSchema#string"/>
        <rdfs:comment>Prefix of the XML namespace.</rdfs:comment>
        <rdfs:isDefinedBy rdf:resource="https://w3id.org/yang/server"/>
        <rdfs:label>namespace prefix</rdfs:label>
    </owl:DatatypeProperty>
    


    <!-- https://w3id.org/yang/server#namespaceURL -->


    <owl:DatatypeProperty rdf:about="https://w3id.org/yang/server#namespaceURL">
        <rdfs:domain rdf:resource="https://w3id.org/yang/server#Namespace"/>
        <rdfs:range rdf:resource="http://www.w3.org/2001/XMLSchema#anyURI"/>
        <rdfs:comment>URL of the XML namespace.</rdfs:comment>
        <rdfs:isDefinedBy rdf:resource="https://w3id.org/yang/server"/>
        <rdfs:label>namespace url</rdfs:label>
    </owl:DatatypeProperty>
    


    <!-- https://w3id.org/yang/server#password -->


    <owl:DatatypeProperty rdf:about="https://w3id.org/yang/server#password">
        <rdfs:domain rdf:resource="https://w3id.org/yang/server#YangServer"/>
        <rdfs:range rdf:resource="http://www.w3.org/2001/XMLSchema#string"/>
        <rdfs:comment>Password for accessing the YANG server.</rdfs:comment>
        <rdfs:isDefinedBy rdf:resource="https://w3id.org/yang/server"/>
        <rdfs:label>password</rdfs:label>
    </owl:DatatypeProperty>
    


    <!-- https://w3id.org/yang/server#subtreeValue -->


    <owl:DatatypeProperty rdf:about="https://w3id.org/yang/server#subtreeValue">
        <rdfs:subPropertyOf rdf:resource="https://w3id.org/yang/server#filterValue"/>
        <rdfs:domain rdf:resource="https://w3id.org/yang/server#SubtreeFilter"/>
        <rdfs:range rdf:resource="http://www.w3.org/1999/02/22-rdf-syntax-ns#XMLLiteral"/>
        <rdfs:comment>XML Subtree filter used to access YANG data of the NETCONF server.</rdfs:comment>
        <rdfs:isDefinedBy rdf:resource="https://w3id.org/yang/server"/>
        <rdfs:label>subtree value</rdfs:label>
    </owl:DatatypeProperty>
    


    <!-- https://w3id.org/yang/server#username -->


    <owl:DatatypeProperty rdf:about="https://w3id.org/yang/server#username">
        <rdfs:domain rdf:resource="https://w3id.org/yang/server#YangServer"/>
        <rdfs:range rdf:resource="http://www.w3.org/2001/XMLSchema#string"/>
        <rdfs:comment>Username for accessing the YANG server.</rdfs:comment>
        <rdfs:isDefinedBy rdf:resource="https://w3id.org/yang/server"/>
        <rdfs:label>username</rdfs:label>
    </owl:DatatypeProperty>
    


    <!-- https://w3id.org/yang/server#xpathValue -->


    <owl:DatatypeProperty rdf:about="https://w3id.org/yang/server#xpathValue">
        <rdfs:subPropertyOf rdf:resource="https://w3id.org/yang/server#filterValue"/>
        <rdfs:domain rdf:resource="https://w3id.org/yang/server#XPathFilter"/>
        <rdfs:range rdf:resource="http://www.w3.org/2001/XMLSchema#string"/>
        <vann:example>/ietf-interfaces:interfaces-state/interface</vann:example>
        <rdfs:comment>XPath expression used to access YANG data of the YANG server.</rdfs:comment>
        <rdfs:isDefinedBy rdf:resource="https://w3id.org/yang/server"/>
        <rdfs:label>xpath value</rdfs:label>
    </owl:DatatypeProperty>
    


    <!-- 
    ///////////////////////////////////////////////////////////////////////////////////////
    //
    // Classes
    //
    ///////////////////////////////////////////////////////////////////////////////////////
     -->


    


    <!-- http://qudt.org/schema/qudt/Unit -->


    <owl:Class rdf:about="http://qudt.org/schema/qudt/Unit">
        <rdfs:isDefinedBy rdf:resource="http://qudt.org/2.1/schema/qudt"/>
        <rdfs:label>Unit</rdfs:label>
    </owl:Class>
    


    <!-- https://w3id.org/yang/server#CandidateDatastore -->


    <owl:Class rdf:about="https://w3id.org/yang/server#CandidateDatastore">
        <rdfs:subClassOf rdf:resource="https://w3id.org/yang/server#ConventionalDatastore"/>
        <rdfs:comment>A configuration datastore that can be manipulated without impacting the device&apos;s running configuration datastore and that can be committed to the running configuration datastore.</rdfs:comment>
        <rdfs:isDefinedBy rdf:resource="https://w3id.org/yang/server"/>
        <rdfs:label>Candidate Datastore</rdfs:label>
        <rdfs:seeAlso rdf:resource="https://datatracker.ietf.org/doc/rfc8342"/>
    </owl:Class>
    


    <!-- https://w3id.org/yang/server#ConventionalDatastore -->


    <owl:Class rdf:about="https://w3id.org/yang/server#ConventionalDatastore">
        <rdfs:subClassOf rdf:resource="https://w3id.org/yang/server#Datastore"/>
        <rdfs:comment>One of the following set of configuration datastores: &lt;running&gt;, &lt;startup&gt;, &lt;candidate&gt;, and &lt;intended&gt;.  These datastores share a common datastore schema, and protocol operations allow copying data between these datastores. The term &quot;conventional&quot; is chosen as a generic umbrella term for these datastores.</rdfs:comment>
        <rdfs:isDefinedBy rdf:resource="https://w3id.org/yang/server"/>
        <rdfs:label>Conventional Datastore</rdfs:label>
        <rdfs:seeAlso rdf:resource="https://datatracker.ietf.org/doc/rfc8342"/>
    </owl:Class>
    


    <!-- https://w3id.org/yang/server#Datastore -->


    <owl:Class rdf:about="https://w3id.org/yang/server#Datastore">
        <rdfs:comment>A conceptual place to store and access information. A datastore might be implemented, for example, using files, a database, flash memory locations, or combinations thereof. A datastore maps to an instantiated YANG data tree.</rdfs:comment>
        <rdfs:isDefinedBy rdf:resource="https://w3id.org/yang/server"/>
        <rdfs:label>Datastore</rdfs:label>
        <rdfs:seeAlso rdf:resource="https://datatracker.ietf.org/doc/rfc8342"/>
    </owl:Class>
    


    <!-- https://w3id.org/yang/server#DynamicDatastore -->


    <owl:Class rdf:about="https://w3id.org/yang/server#DynamicDatastore">
        <rdfs:subClassOf rdf:resource="https://w3id.org/yang/server#Datastore"/>
        <rdfs:comment>A configuration datastore holding configuration obtained dynamically during the operation of a device through interaction with other systems, rather than through one of the conventional configuration datastores.</rdfs:comment>
        <rdfs:isDefinedBy rdf:resource="https://w3id.org/yang/server"/>
        <rdfs:label>Dynamic Datastore</rdfs:label>
        <rdfs:seeAlso rdf:resource="https://datatracker.ietf.org/doc/rfc8342"/>
    </owl:Class>
    


    <!-- https://w3id.org/yang/server#Filter -->


    <owl:Class rdf:about="https://w3id.org/yang/server#Filter">
        <rdfs:comment>Evaluation criteria that may be applied to fetch data from a given YANG server.</rdfs:comment>
        <rdfs:isDefinedBy rdf:resource="https://w3id.org/yang/server"/>
        <rdfs:label>Filter</rdfs:label>
        <rdfs:seeAlso rdf:resource="https://datatracker.ietf.org/doc/rfc6241"/>
    </owl:Class>
    


    <!-- https://w3id.org/yang/server#IntendedDatastore -->


    <owl:Class rdf:about="https://w3id.org/yang/server#IntendedDatastore">
        <rdfs:subClassOf rdf:resource="https://w3id.org/yang/server#ConventionalDatastore"/>
        <rdfs:comment>A configuration datastore holding the complete intended configuration of the device. This represents the configuration after all configuration transformations to &lt;running&gt; have been performed and is the configuration that the system attempts to apply.</rdfs:comment>
        <rdfs:isDefinedBy rdf:resource="https://w3id.org/yang/server"/>
        <rdfs:label>Intended Datastore</rdfs:label>
        <rdfs:seeAlso rdf:resource="https://datatracker.ietf.org/doc/rfc8342"/>
    </owl:Class>
    


    <!-- https://w3id.org/yang/server#Namespace -->


    <owl:Class rdf:about="https://w3id.org/yang/server#Namespace">
        <rdfs:comment>Represents an XML namespace used in the XPath expression.</rdfs:comment>
        <rdfs:isDefinedBy rdf:resource="https://w3id.org/yang/server"/>
        <rdfs:label>Namespace</rdfs:label>
    </owl:Class>
    


    <!-- https://w3id.org/yang/server#NetconfCapability -->


    <owl:Class rdf:about="https://w3id.org/yang/server#NetconfCapability">
        <rdfs:comment>NETCONF capability.</rdfs:comment>
        <rdfs:isDefinedBy rdf:resource="https://w3id.org/yang/server"/>
        <rdfs:label>Netconf Capability</rdfs:label>
        <rdfs:seeAlso rdf:resource="https://datatracker.ietf.org/doc/rfc6241"/>
    </owl:Class>
    


    <!-- https://w3id.org/yang/server#NetconfServer -->


    <owl:Class rdf:about="https://w3id.org/yang/server#NetconfServer">
        <rdfs:subClassOf rdf:resource="https://w3id.org/yang/server#YangServer"/>
        <rdfs:comment>YANG server that can be managed via the NETCONF protocol.</rdfs:comment>
        <rdfs:isDefinedBy rdf:resource="https://w3id.org/yang/server"/>
        <rdfs:label>Netconf Server</rdfs:label>
        <rdfs:seeAlso rdf:resource="https://datatracker.ietf.org/doc/rfc6241"/>
    </owl:Class>
    


    <!-- https://w3id.org/yang/server#OnChangeSubscription -->


    <owl:Class rdf:about="https://w3id.org/yang/server#OnChangeSubscription">
        <rdfs:subClassOf rdf:resource="https://w3id.org/yang/server#Subscription"/>
        <rdfs:comment>A datastore subscription with updates that are triggered when changes in subscribed datastore nodes are detected.</rdfs:comment>
        <rdfs:isDefinedBy rdf:resource="https://w3id.org/yang/server"/>
        <rdfs:label>On-change Subscription</rdfs:label>
        <rdfs:seeAlso rdf:resource="https://datatracker.ietf.org/doc/rfc8641"/>
    </owl:Class>
    


    <!-- https://w3id.org/yang/server#OperationalDatastore -->


    <owl:Class rdf:about="https://w3id.org/yang/server#OperationalDatastore">
        <rdfs:subClassOf rdf:resource="https://w3id.org/yang/server#Datastore"/>
        <rdfs:comment>A datastore holding the complete operational state of the device.</rdfs:comment>
        <rdfs:isDefinedBy rdf:resource="https://w3id.org/yang/server"/>
        <rdfs:label>Operational Datastore</rdfs:label>
        <rdfs:seeAlso rdf:resource="https://datatracker.ietf.org/doc/rfc8342"/>
    </owl:Class>
    


    <!-- https://w3id.org/yang/server#Period -->


    <owl:Class rdf:about="https://w3id.org/yang/server#Period">
        <rdfs:comment>Represents the period interval with which to report updates in a periodic subscription.</rdfs:comment>
        <rdfs:isDefinedBy rdf:resource="https://w3id.org/yang/server"/>
        <rdfs:label>Period</rdfs:label>
        <rdfs:seeAlso rdf:resource="https://datatracker.ietf.org/doc/rfc8641"/>
    </owl:Class>
    


    <!-- https://w3id.org/yang/server#PeriodicSubscription -->


    <owl:Class rdf:about="https://w3id.org/yang/server#PeriodicSubscription">
        <rdfs:subClassOf rdf:resource="https://w3id.org/yang/server#Subscription"/>
        <rdfs:comment>A datastore subscription with updates that are triggered periodically according to some time interval.</rdfs:comment>
        <rdfs:isDefinedBy rdf:resource="https://w3id.org/yang/server"/>
        <rdfs:label>Periodic Subscription</rdfs:label>
        <rdfs:seeAlso rdf:resource="https://datatracker.ietf.org/doc/rfc8641"/>
    </owl:Class>
    


    <!-- https://w3id.org/yang/server#Query -->


    <owl:Class rdf:about="https://w3id.org/yang/server#Query">
        <rdfs:comment>Represents a query operation to a YANG server using the corresponding network management protocol.</rdfs:comment>
        <rdfs:isDefinedBy rdf:resource="https://w3id.org/yang/server"/>
        <rdfs:label>Query</rdfs:label>
        <rdfs:seeAlso rdf:resource="https://datatracker.ietf.org/doc/rfc6241"/>
    </owl:Class>
    


    <!-- https://w3id.org/yang/server#RunningDatastore -->


    <owl:Class rdf:about="https://w3id.org/yang/server#RunningDatastore">
        <rdfs:subClassOf rdf:resource="https://w3id.org/yang/server#ConventionalDatastore"/>
        <rdfs:comment>A configuration datastore holding the current configuration of the device.  It may include configuration that requires further transformations before it can be applied.</rdfs:comment>
        <rdfs:isDefinedBy rdf:resource="https://w3id.org/yang/server"/>
        <rdfs:label>Running Datastore</rdfs:label>
        <rdfs:seeAlso rdf:resource="https://datatracker.ietf.org/doc/rfc8342"/>
    </owl:Class>
    


    <!-- https://w3id.org/yang/server#StartupDatastore -->


    <owl:Class rdf:about="https://w3id.org/yang/server#StartupDatastore">
        <rdfs:subClassOf rdf:resource="https://w3id.org/yang/server#ConventionalDatastore"/>
        <rdfs:comment>A configuration datastore holding the configuration loaded by the device into the running configuration datastore when it boots.</rdfs:comment>
        <rdfs:isDefinedBy rdf:resource="https://w3id.org/yang/server"/>
        <rdfs:label>Startup Datastore</rdfs:label>
        <rdfs:seeAlso rdf:resource="https://datatracker.ietf.org/doc/rfc8342"/>
    </owl:Class>
    


    <!-- https://w3id.org/yang/server#Subscription -->


    <owl:Class rdf:about="https://w3id.org/yang/server#Subscription">
        <rdfs:comment>Represents a subscription operation to a YANG server using the corresponding network management protocol.</rdfs:comment>
        <rdfs:isDefinedBy rdf:resource="https://w3id.org/yang/server"/>
        <rdfs:label>Subscription</rdfs:label>
        <rdfs:seeAlso rdf:resource="https://datatracker.ietf.org/doc/rfc8641"/>
    </owl:Class>
    


    <!-- https://w3id.org/yang/server#SubtreeFilter -->


    <owl:Class rdf:about="https://w3id.org/yang/server#SubtreeFilter">
        <rdfs:subClassOf rdf:resource="https://w3id.org/yang/server#Filter"/>
        <rdfs:comment>Evaluation criteria based on XML subtree expression.</rdfs:comment>
        <rdfs:isDefinedBy rdf:resource="https://w3id.org/yang/server"/>
        <rdfs:label>Subtree Filter</rdfs:label>
        <rdfs:seeAlso rdf:resource="https://datatracker.ietf.org/doc/rfc6241"/>
    </owl:Class>
    


    <!-- https://w3id.org/yang/server#XPathFilter -->


    <owl:Class rdf:about="https://w3id.org/yang/server#XPathFilter">
        <rdfs:subClassOf rdf:resource="https://w3id.org/yang/server#Filter"/>
        <rdfs:comment>Evaluation criteria based on XPath expression.</rdfs:comment>
        <rdfs:isDefinedBy rdf:resource="https://w3id.org/yang/server"/>
        <rdfs:label>XPath Filter</rdfs:label>
        <rdfs:seeAlso rdf:resource="https://datatracker.ietf.org/doc/rfc6241"/>
    </owl:Class>
    


    <!-- https://w3id.org/yang/server#YangServer -->


    <owl:Class rdf:about="https://w3id.org/yang/server#YangServer">
        <rdfs:comment>An entity that provides access to YANG-defined data to a client, over some network management protocol.</rdfs:comment>
        <rdfs:isDefinedBy rdf:resource="https://w3id.org/yang/server"/>
        <rdfs:label>Yang Server</rdfs:label>
        <rdfs:seeAlso rdf:resource="https://datatracker.ietf.org/doc/rfc7950"/>
    </owl:Class>
    


    <!-- 
    ///////////////////////////////////////////////////////////////////////////////////////
    //
    // Individuals
    //
    ///////////////////////////////////////////////////////////////////////////////////////
     -->


    


    <!-- https://w3id.org/yang/server#CandidateCapability -->


    <owl:NamedIndividual rdf:about="https://w3id.org/yang/server#CandidateCapability">
        <rdf:type rdf:resource="https://w3id.org/yang/server#NetconfCapability"/>
        <terms:identifier>urn:ietf:params:netconf:capability:candidate:1.0</terms:identifier>
        <rdfs:comment>The candidate configuration capability, `:candidate`, indicates that the device supports a candidate configuration datastore, which is used to hold configuration data that can be manipulated without impacting the device&apos;s current configuration.</rdfs:comment>
        <rdfs:isDefinedBy rdf:resource="https://w3id.org/yang/server"/>
        <rdfs:label>Candidate Capability</rdfs:label>
        <rdfs:seeAlso rdf:resource="https://datatracker.ietf.org/doc/html/rfc6241#section-8.3"/>
    </owl:NamedIndividual>
    


    <!-- https://w3id.org/yang/server#ConfirmedCommitCapability -->


    <owl:NamedIndividual rdf:about="https://w3id.org/yang/server#ConfirmedCommitCapability">
        <rdf:type rdf:resource="https://w3id.org/yang/server#NetconfCapability"/>
        <terms:identifier>urn:ietf:params:netconf:capability:confirmed-commit:1.1</terms:identifier>
        <rdfs:comment>The `:confirmed-commit:1.1` capability indicates that the server will support the `&lt;cancel-commit&gt;` operation and the `&lt;confirmed&gt;`, `&lt;confirm-timeout&gt;`, `&lt;persist&gt;`, and `&lt;persist-id&gt;` parameters for the `&lt;commit&gt;` operation.</rdfs:comment>
        <rdfs:isDefinedBy rdf:resource="https://w3id.org/yang/server"/>
        <rdfs:label>Confirmed Commit Capability</rdfs:label>
        <rdfs:seeAlso rdf:resource="https://datatracker.ietf.org/doc/html/rfc6241#section-8.4"/>
    </owl:NamedIndividual>
    


    <!-- https://w3id.org/yang/server#DistinctStartupCapability -->


    <owl:NamedIndividual rdf:about="https://w3id.org/yang/server#DistinctStartupCapability">
        <rdf:type rdf:resource="https://w3id.org/yang/server#NetconfCapability"/>
        <terms:identifier>urn:ietf:params:netconf:capability:startup:1.0</terms:identifier>
        <rdfs:comment>The device supports separate running and startup configuration datastores. The startup configuration is loaded by the device when it boots.</rdfs:comment>
        <rdfs:isDefinedBy rdf:resource="https://w3id.org/yang/server"/>
        <rdfs:label>Distinct Startup Capability</rdfs:label>
        <rdfs:seeAlso rdf:resource="https://datatracker.ietf.org/doc/html/rfc6241#section-8.7"/>
    </owl:NamedIndividual>
    


    <!-- https://w3id.org/yang/server#RollbackOnErrorCapability -->


    <owl:NamedIndividual rdf:about="https://w3id.org/yang/server#RollbackOnErrorCapability">
        <rdf:type rdf:resource="https://w3id.org/yang/server#NetconfCapability"/>
        <terms:identifier>urn:ietf:params:netconf:capability:rollback-on-error:1.0</terms:identifier>
        <rdfs:comment>This capability indicates that the server will support the `rollback-on-error` value in the `&lt;error-option&gt;` parameter to the `&lt;edit-config&gt;` operation.</rdfs:comment>
        <rdfs:isDefinedBy rdf:resource="https://w3id.org/yang/server"/>
        <rdfs:label>Rollback-on-Error Capability</rdfs:label>
        <rdfs:seeAlso rdf:resource="https://datatracker.ietf.org/doc/html/rfc6241#section-8.5"/>
    </owl:NamedIndividual>
    


    <!-- https://w3id.org/yang/server#UrlCapability -->


    <owl:NamedIndividual rdf:about="https://w3id.org/yang/server#UrlCapability">
        <rdf:type rdf:resource="https://w3id.org/yang/server#NetconfCapability"/>
        <terms:identifier>urn:ietf:params:netconf:capability:url:1.0</terms:identifier>
        <rdfs:comment>The NETCONF peer has the ability to accept the `&lt;url&gt;` element in `&lt;source&gt;` and `&lt;target&gt;` parameters. The capability is further identified by URL arguments indicating the URL schemes supported.</rdfs:comment>
        <rdfs:isDefinedBy rdf:resource="https://w3id.org/yang/server"/>
        <rdfs:label>URL Capability</rdfs:label>
        <rdfs:seeAlso rdf:resource="https://datatracker.ietf.org/doc/html/rfc6241#section-8.8"/>
    </owl:NamedIndividual>
    


    <!-- https://w3id.org/yang/server#ValidationCapability -->


    <owl:NamedIndividual rdf:about="https://w3id.org/yang/server#ValidationCapability">
        <rdf:type rdf:resource="https://w3id.org/yang/server#NetconfCapability"/>
        <terms:identifier>urn:ietf:params:netconf:capability:validate:1.1</terms:identifier>
        <rdfs:comment>Validation consists of checking a complete configuration for syntactical and semantic errors before applying the configuration to the device.</rdfs:comment>
        <rdfs:isDefinedBy rdf:resource="https://w3id.org/yang/server"/>
        <rdfs:label>Validation Capability</rdfs:label>
        <rdfs:seeAlso rdf:resource="https://datatracker.ietf.org/doc/html/rfc6241#section-8.6"/>
    </owl:NamedIndividual>
    


    <!-- https://w3id.org/yang/server#WritableRunningCapability -->


    <owl:NamedIndividual rdf:about="https://w3id.org/yang/server#WritableRunningCapability">
        <rdf:type rdf:resource="https://w3id.org/yang/server#NetconfCapability"/>
        <terms:identifier>urn:ietf:params:netconf:capability:writable-running:1.0</terms:identifier>
        <rdfs:comment>The `:writable-running` capability indicates that the device supports direct writes to the `&lt;running&gt;` configuration datastore. In other words, the device supports `&lt;edit-config&gt;` and `&lt;copy-config&gt;` operations where the `&lt;running&gt;` configuration is the target.</rdfs:comment>
        <rdfs:isDefinedBy rdf:resource="https://w3id.org/yang/server"/>
        <rdfs:label>Writable Running Capability</rdfs:label>
        <rdfs:seeAlso rdf:resource="https://datatracker.ietf.org/doc/html/rfc6241#section-8.2"/>
    </owl:NamedIndividual>
    


    <!-- https://w3id.org/yang/server#XpathCapability -->


    <owl:NamedIndividual rdf:about="https://w3id.org/yang/server#XpathCapability">
        <rdf:type rdf:resource="https://w3id.org/yang/server#NetconfCapability"/>
        <terms:identifier>urn:ietf:params:netconf:capability:xpath:1.0</terms:identifier>
        <rdfs:comment>The XPath capability indicates that the NETCONF peer supports the use of XPath expressions in the `&lt;filter&gt;` element.</rdfs:comment>
        <rdfs:isDefinedBy rdf:resource="https://w3id.org/yang/server"/>
        <rdfs:label>XPath Capability</rdfs:label>
        <rdfs:seeAlso rdf:resource="https://datatracker.ietf.org/doc/html/rfc6241#section-8.9"/>
    </owl:NamedIndividual>
    


    <!-- https://w3id.org/yang/server#YangLibraryCapability -->


    <owl:NamedIndividual rdf:about="https://w3id.org/yang/server#YangLibraryCapability">
        <rdf:type rdf:resource="https://w3id.org/yang/server#NetconfCapability"/>
        <terms:identifier>urn:ietf:params:netconf:capability:yang-library:1.1</terms:identifier>
        <rdfs:comment>NETCONF capability that indicates that the NETCONF server implements YANG Library.</rdfs:comment>
        <rdfs:isDefinedBy rdf:resource="https://w3id.org/yang/server"/>
        <rdfs:label>Yang Library Capability</rdfs:label>
        <rdfs:seeAlso rdf:resource="https://datatracker.ietf.org/doc/html/rfc8526"/>
    </owl:NamedIndividual>
</rdf:RDF>



<!-- Generated by the OWL API (version 5.1.18) https://github.com/owlcs/owlapi/ -->


